Clean/Orchard/Ecc/Defs.lean
@@ -8,7 +8,7 @@ import Mathlib.Tactic
 Some definitions useful for circuits involving points
 -/
 namespace Orchard
-variable {F : Type} [Field F]
+variable {F : Type} [FiniteField F]
 
 structure CurrentNext (F : Type) where
   curr : F
